proof/invariants/UpdateShadow1Structure.v
@@ -683,11 +683,11 @@ Qed.
 Lemma getConfigTablesLinkedListsAddDerivation sh3  (descChild : vaddr) table idx entry
  (s : state) flag:
 lookup table idx (memory s) beqPage beqIndex = Some (VE entry) -> 
-getTrdShadows sh3
+getLLPages sh3
   {|
   currentPartition := currentPartition s;
   memory := add table idx (VE {| pd := flag; va := descChild |}) (memory s) beqPage beqIndex |} (nbPage+1) =
-getTrdShadows sh3 s (nbPage+1).
+getLLPages sh3 s (nbPage+1).
 Proof.
 revert sh3.
 induction (nbPage+1);trivial.
